src/Std/Data/Iterators/Lemmas.lean
@@ -9,3 +9,4 @@ import Std.Data.Iterators.Lemmas.Monadic
 import Std.Data.Iterators.Lemmas.Consumers
 import Std.Data.Iterators.Lemmas.Combinators
 import Std.Data.Iterators.Lemmas.Producers
+import Std.Data.Iterators.Lemmas.Equivalence
